Urm.lean
@@ -5,5 +5,6 @@ import Urm.Execution
 import Urm.Shift
 import Urm.Computable
 import Urm.Composition
+import Urm.UnaryComposition
 import Urm.BinaryUnaryComposition
 import Urm.Examples
